#+title: Derivations
#+author: Erik An
#+email: obluda2173@gmail.com
#+date: <2025-12-06>
#+lastmod: <2025-12-06 06:54>
#+options: num:t
#+startup: overview

* Given formulas to use

$esticatePrice(mileage) = \theta_0 + (\theta_1 \times mileage)$

$tmp\theta_0 = learningRate \times \dfrac{1}{m} \times \sum_{i=0}^{m-1} (estimatePrice(mileage[i]) - price[i])$

$tmp\theta_1 = learningRate \times \dfrac{1}{m} \times \sum_{i=0}^{m-1} (estimatePrice(mileage[i]) - price[i]) \times mileage[i]$

* Mean Square Error

$MSE = \dfrac{1}{n} \times \sum_{i=1}^{n} (Y_i - \hat{Y_i})^2$

where:
- $n$ :: amount of observation quantities
- $Y_i$ :: observed quantities
- $\hat{Y_i}$ :: predicted quantities

Hence,

$MSE' = \dfrac{2}{n} \times \sum_{i=1}^{n} (Y_i - \hat{Y_i})$

which looks familiar, since it basically is the given formulas.
